hwqueue/HWQI.v
@@ -1,4 +1,4 @@
-Require Export CRIS ImpPrelude HWQHeader SchHeader MemHeader.
+Require Export CRIS ImpPrelude HWQHeader SchHeader MemHeader ProphecyHeader.
 (** * Implementation of the queue operations ********************************)
 
 Module HWQI. Section HWQI.
@@ -98,10 +98,13 @@ Module HWQI. Section HWQI.
         𝒴;;; let range := Z.to_nat (Z.min sz back) in
         dequeue_aux (Vptr (qblk, qofs)) range range) ().
 
+  Definition mask : emask :=
+    CFilter.msk_filter_in (MemHdr.exports ∪ SchHdr.exports) (msk_real (msk_scp [] msk_true)).
+  
   Definition fnsems : fnsemmap :=
-    {[fid HWQHdr.new_queue # (msk_real (msk_scp [] msk_true), (None, cfunU new_queue));
-      fid HWQHdr.enqueue   # (msk_real (msk_scp [] msk_true), (None, cfunU enqueue));
-      fid HWQHdr.dequeue   # (msk_real (msk_scp [] msk_true), (None, cfunU dequeue))]}.
+    {[fid HWQHdr.new_queue # (mask, (None, cfunU new_queue));
+      fid HWQHdr.enqueue   # (mask, (None, cfunU enqueue));
+      fid HWQHdr.dequeue   # (mask, (None, cfunU dequeue))]}.
 
   Program Definition Mod : SMod.t := {|
     SMod.scopes := [];
@@ -111,4 +114,9 @@ Module HWQI. Section HWQI.
   Solve All Obligations with mod_tac.
 
   Definition t := SMod.to_mod ∅ Mod.
+
+  Lemma filter_prophecy mn:
+    CFilter.filter (Prophecy.exports mn) t = t.
+  Proof. cfilter_solver. Qed.
+  
 End HWQI. End HWQI.
