hwqueue/HWQIA.v
@@ -3,40 +3,28 @@ Require Export CallFilter MemA SchA ProphecyA.
 Require Export HWQRA.
 Require Import MemI MemIAproof MemTactics.
 Require Import ProphecyI ProphecyFacts.
-Require Import HelpingTactics SchI SchTactics.
+Require Import HelpingTactics HelpingFacts SchI SchTactics.
 Require Import HWQI HWQP HWQA HWQIANewQueue HWQIAEnqueue HWQIADequeue.
 
 Module HWQPM. Section HWQPM.
   Context `{!crisG Γ Σ α β τ Hinv Hsub, !concGS, !memGS, !prophGS, !schGS, !hwqG}.
-  Context (mn : string).
+  Context (mnp mnh : string).
   Context (N : namespace) (sp_mem : specmap).
 
-  Definition Ist : ist_type Σ := λ st_src st_tgt,
-    (IstHelp mn st_src st_tgt ∗
-    ∃ (X : gset val),
-      free_id (λ x, (x.1 = "hwq" ∧ match (x.2↓↓) with | Some x => x ∉ X | None => True end)%type) ∗
-      [∗ set] x ∈ X,
-        □ ∃ blk ofs nx, ⌜x = Vptr (blk, ofs)⌝ ∗
-          ∀ X, helping_auth 1 X =| nx, ↑N |={↑N, ∅}=∗ ∃ v, (blk, ofs) ↦ v)%I.
-  Definition IstFull : ist_type Σ :=
-    IstProd (IstSB (Mod.scopes (HWQP.t mn) ++ Mod.scopes (HelpingDummy.t mn)) Ist) IstEq.
-
   Notation sp := (SchA.sp ∅ (↑N)).
-  Notation HWQM := (HWQM.t N mn).
-  Notation HWQP := (HWQP.t mn).
-  Notation HelpOn := (HelpingOn.t mn HWQM.jobCode sp).
-  Notation HelpDummy := (HelpingDummy.t mn).
+  Notation HWQM := (HWQM.t N mnh).
+  Notation HWQP := (HWQP.t mnp).
+  Notation HelpOn := (HelpingOn.t mnh HWQM.jobCode sp).
+  Notation HelpDummy := (HelpingDummy.t mnh).
   Notation MemA := (MemA.t sp_mem).
-  Notation ProphA := (ProphecyA.t mn ∅).
+  Notation ProphA := (ProphecyA.t mnp ∅).
 
   Lemma ctxr :
     ctx_refines
-      ((HWQM.t N mn ★ HelpingOn.t mn (HWQM.jobCode) sp) ★ MemA.t sp_mem ★ ProphecyA.t mn ∅,
-          helping_auth 1 ∅ ∗ free_id top1)%I
-      ((HWQP.t mn   ★ HelpingDummy.t mn)                ★ MemA.t sp_mem ★ ProphecyA.t mn ∅,
-          emp)%I.
+      ((HWQM ★ HelpOn)     ★ MemA ★ ProphA, helping_auth 1 ∅ ∗ free_id top1)%I
+      ((HWQP ★ HelpDummy)  ★ MemA ★ ProphA, emp)%I.
   Proof.
-    eapply main_adequacy with (Ist := IstFull).
+    eapply main_adequacy with (Ist := HWQIAInv.IstFull mnp mnh N).
     cStartModSim.
     { apply simF_new_queue. }
     { apply simF_enqueue. }
@@ -64,59 +52,109 @@ Module HWQPM. Section HWQPM.
   Qed.
 End HWQPM. End HWQPM.
 
+Module HWQMA. Section HWQMA.
+  Context `{!crisG Γ Σ α β τ Hinv Hsub, !concGS, !memGS, !prophGS, !schGS, !hwqG}.
+  Context (mnp mnh : string).
+  Context (N : namespace) (sp_user sp : specmap).
+  Hypothesis (SchSP: SchA.sp sp_user (↑N) ⊆ sp).
+  
+  Lemma ctxr:
+    ctx_refines
+      (HWQA.t N sp, emp%I)
+      (HWQM.t N mnh ★ ProphecyA.t mnp ∅ ★ HelpingOff.t mnh HWQM.jobCode (SchA.sp ∅ (↑N)), emp%I).
+  Proof.
+    eapply main_adequacy. instantiate (1:=λ _ _, True%I).
+    cStartModSim; ss.
+    - cStartFunSim. rewrite /HWQA.new_queue.
+      cStepsS. cForcesT. iFrame. cStepsT. destruct Any.downcast; cStepsS; ss.
+      cStepsT. sYieldII "IST". sYieldS. cForcesS. iFrame. cStep. done.
+    - cStartFunSim. rewrite /HWQA.enqueue /HWQM.enqueue /atomic_body.
+      cStepsS. cStepsT. cForcesT. iFrame. cStepsT.
+      destruct _q as [[? ?] [[[[? ?] ?] ?] ?]]. sYieldII "IST".
+      cInlineT. cStepsT. rewrite /HelpingOff.run. cStepsT. sYieldII "IST".
+      sYieldS. cStepsS. cForcesT. iFrame. cStepsT. cForcesS. iFrame.
+      cStepsS. sYieldII "IST".
+      iApply wsim_reset.
+      cCoind CIH g' __ with st_src st_tgt. iIntros "IST".
+      unfoldIterT. cStepsT. case_match.
+      { cStepsT. cInlineT. cStepsT. rewrite /HelpingOff.help. cStepsT.
+        sYieldII "IST". cByCoind CIH; iFrame.
+      }
+      cStepsT. sYieldII "IST". sYieldS. cForceS; iFrame. cStep. done.
+    - cStartFunSim. rewrite /HWQA.dequeue /HWQM.dequeue /atomic_body.
+      cStepsS. cStepsT. cForcesT. iFrame. cStepsT.
+      sYieldII "IST". sYieldS.
+      destruct _q as [[? ?] [[[? ?] ?] ?]]. cStepsS. cForcesT; iFrame.
+      cStepsT. cForcesS; iFrame. cStepsS.
+      sYieldII "IST". sYieldS. cForcesS; iFrame.
+      cStep; done.
+  Qed.
+
+End HWQMA. End HWQMA.
+
 Module HWQIA. Section HWQIA.
   Context `{!crisG Γ Σ α β τ Hinv Hsub, !concGS, !schGS, !hwqG, !memGS, !prophGS}.
 
-  Lemma ctxr (ctx : Mod.t) (N : namespace) (sp_user sp sp_mem : specmap) csl genv :
+  Lemma refines (ctx : Mod.t) (N : namespace) (sp_user sp sp_mem : specmap) csl genv :
     SchA.sp sp_user (↑N) ⊆ sp →
     real_mod ctx →
     refines
       (HWQA.t N sp ★ MemA.t sp_mem   ★ SchI.t ★ ctx,
-        MemA.init_cond csl genv ∗ ProphecyA.initial_cond ∗ helping_auth 1 ∅ ∗ free_id top1)%I
+       MemA.init_cond csl genv ∗ ProphecyA.initial_cond ∗ helping_auth 1 ∅ ∗ free_id top1)%I
       (HWQI.t      ★ MemI.t csl genv ★ SchI.t ★ ctx,
-        emp%I).
+       emp%I).
   Proof.
     intros Hsch Hreal.
-    eapply helping_prophecy_refines; eauto.
-    { apply HWQIP.ctxr. }
-    { intros mn; etrans; cycle 1.
-      { rewrite assoc; apply HWQPM.ctxr with (N:=N). }
-      rewrite assoc //.
-    }
-    { intros mn; eapply main_adequacy.
-      instantiate (1:=λ _ _, True%I).
-      cStartModSim; first done; cStartFunSim; ss.
-      { cStepsS. cForcesT. iFrame. cStepsT. destruct Any.downcast; cStepsS; ss.
-        rewrite /HWQA.new_queue.
-        cStepsT. cStepsS. sYieldII "IST". sYieldS. cForcesS. iFrame. cStep. done.
+
+    set (allmds := HWQA.t N sp ★ MemA.t sp_mem ★ HWQI.t ★ MemI.t csl genv ★ SchI.t ★ ctx).
+    set (sz := S (max
+                 (maxlen (elements (get_fids (dom (Mod.fnsems allmds)))))
+                 (maxlen (Mod.scopes allmds)))).
+
+    etrans; cycle 1.
+    { rewrite assoc.
+      eapply prophecy_refines with (sz:=sz) (mdm := λ mn, HWQP.t mn ★ MemI.t csl genv).
+      { intros Q. rewrite !CFilter.filter_app.
+        etrans; cycle 1.
+        { eapply ctxr_refines.
+          ctxr_rotate. ctxr_drop. ctxr_rotate. do 2 ctxr_drop.
+          rewrite HWQI.filter_prophecy. apply HWQIP.ctxr. }
+        rewrite MemI.filter_prophecy.
+        evar_at_last_1; [refl|f_equal]. mod_eq_solver.
       }
-      { rewrite /HWQA.enqueue /HWQM.enqueue /atomic_body.
-        cStepsS. cStepsT. cForcesT. iFrame. cStepsT.
-        destruct _q as [[? ?] [[[[? ?] ?] ?] ?]]. sYieldII "IST".
-        cInlineT. cStepsT. rewrite /HelpingOff.run. cStepsT. sYieldII "IST".
-        sYieldS. cStepsS. cForcesT. iFrame. cStepsT. cForcesS. iFrame.
-        cStepsS. sYieldII "IST".
-        iApply wsim_reset.
-        cCoind CIH g' __ with st_src st_tgt. iIntros "IST".
-        unfoldIterT. cStepsT. case_match.
-        { cStepsT. cInlineT. cStepsT. rewrite /HelpingOff.help. cStepsT.
-          sYieldII "IST". cByCoind CIH; iFrame.
+      { intros Q. etrans; cycle 1.
+        { eapply ctxr_refines. do 2 ctxr_rotate. do 3 ctxr_drop. apply MemIA.ctxr. }
+        etrans; cycle 1.
+        { rewrite comm -assoc comm.
+          eapply helping_refines
+            with (mA := HWQA.t N sp ★ MemA.t sp_mem)
+                 (mM := λ mnh, HWQM.t N mnh ★ MemA.t sp_mem ★ ProphecyA.t _ ∅).
+          - intros Q0 mnh. eapply ctxr_refines. etrans; cycle 1.
+            { do 2 rewrite CFilter.filter_app.
+              rewrite HWQP.filter_helping MemA.filter_helping ProphecyA.filter_helping.
+              do 3 ctxr_rotate. ctxr_drop. ctxr_swap. rewrite assoc. eapply HWQPM.ctxr.
+            }
+            evar_at_last_1; [refl|f_equal]. mod_eq_solver.
+          - intros Q0 mnh. eapply ctxr_refines. etrans; cycle 1.
+            { ctxr_rotate. ctxr_drop. ctxr_rotate. ctxr_drop. ctxr_rotate.
+              eapply HWQMA.ctxr; et.
+            }
+            evar_at_last_1; [refl|f_equal]. mod_eq_solver.
+          - intros fn IN1 IN2. subst sz allmds.
+            rewrite -elem_of_elements in IN1. eapply elem_of_maxlen in IN1.
+            eapply prophecy_exports_long in IN2. rewrite mname_long_length in IN2.
+            do 3 rewrite Mod.dom_fnsems_add maxlen_get_fids_union in IN1.
+            do 5 rewrite Mod.dom_fnsems_add maxlen_get_fids_union in IN2. nia.
         }
-        cStepsT. sYieldII "IST". sYieldS. cForceS; iFrame. cStep. done.
+        etrans; cycle 1.
+        { eapply ctxr_refines. do 2 ctxr_drop. eapply CFilter.intro_filter. }
+        rewrite !left_id !assoc. refl.
       }
-      { rewrite /HWQA.dequeue /HWQM.dequeue /atomic_body.
-        cStepsS. cStepsT. cForcesT. iFrame. cStepsT.
-        sYieldII "IST". sYieldS.
-        destruct _q as [[? ?] [[[? ?] ?] ?]]. cStepsS. cForcesT; iFrame.
-        cStepsT. cForcesS; iFrame. cStepsS.
-        sYieldII "IST". sYieldS. cForcesS; iFrame.
-        cStep; done.
-      }
+      { rewrite -!assoc. et. }
+      { eapply Mod.real_mod_add; [apply HWQP.real|apply MemI.real]. }
+      { eapply Mod.real_mod_add; et. apply SchI.real. }
     }
-    { intros mn; rewrite /real_mod.
-      let real_tac :=
-        (split; ss; intros ??; destruct excluded_middle_informative; ss) in
-      mod_tac real_tac.
-    }
+    rewrite !left_id -!assoc.
+    eapply ctxr_refines, ctxr_cond_strengthen. iIntros "[$ $]".
   Qed.
 End HWQIA. End HWQIA.
