hwqueue/HWQIANewQueue.v
@@ -9,33 +9,20 @@ From stdpp Require Import streams list.
 
 Section HWQPM.
   Context `{!crisG Γ Σ α β τ Hinv Hsub, !concGS, !schGS, !hwqG, !memGS, !prophGS}.
-  Context (mn : string).
+  Context (mnp mnh: string).
   Context (N : namespace) (sp_mem : specmap).
 
-  Definition Ist : ist_type Σ := λ st_src st_tgt,
-    (IstHelp mn st_src st_tgt ∗
-    ∃ (X : gset val),
-      free_id (λ x, (x.1 = "hwq" ∧ match (x.2↓↓) with | Some x => x ∉ X | None => True end)%type) ∗
-      [∗ set] x ∈ X,
-        □ ∃ blk ofs nx, ⌜x = Vptr (blk, ofs)⌝ ∗
-          ∀ X, helping_auth 1 X =| nx, ↑N |={↑N, ∅}=∗ ∃ v, (blk, ofs) ↦ v)%I.
-  Definition IstFull : ist_type Σ :=
-    IstProd (IstSB (Mod.scopes (HWQP.t mn) ++ Mod.scopes (HelpingDummy.t mn)) Ist) IstEq.
-  Lemma Ist_help : Ist_helping mn IstFull.
-  Proof.
-    iIntros (??) "[% [% [% [% [[-> ->] [[%Ha [[% [[-> ->] ?]] ?]] ->]]]]]]".
-    iModIntro; iExists _, _; iFrame; iSplit; auto.
-    iIntros (?) "$ !>"; iExists _, _, _, _; repeat iSplit; eauto.
-    iPureIntro. set_solver.
-  Qed.
-
   Notation sp := (SchA.sp ∅ (↑N)).
-  Notation HWQM := (HWQM.t N mn).
-  Notation HWQP := (HWQP.t mn).
-  Notation HelpOn := (HelpingOn.t mn HWQM.jobCode sp).
-  Notation HelpDummy := (HelpingDummy.t mn).
+  Notation HWQM := (HWQM.t N mnh).
+  Notation HWQP := (HWQP.t mnp).
+  Notation HelpOn := (HelpingOn.t mnh HWQM.jobCode sp).
+  Notation HelpDummy := (HelpingDummy.t mnh).
   Notation MemA := (MemA.t sp_mem).
-  Notation ProphA := (ProphecyA.t mn ∅).
+  Notation ProphA := (ProphecyA.t mnp ∅).
+  Notation IstFull := (HWQIAInv.IstFull mnp mnh N).
+
+  Local Ltac yield_tac H1 H2 :=
+    sYieldIR H1 H2; [eapply bool_decide_eq_true; set_solver|].
 
   Lemma simF_new_queue : 
     ISim.sim_fun open
@@ -47,13 +34,13 @@ Section HWQPM.
     iDestruct "ASM" as "[TID [-> [-> %Hsz]]]".
     cStepsS. cStepsT.
     rewrite /HWQP.new_queue /HWQA.new_queue.
-    cStepsT. sYieldIR "IST" "TID". sYieldIR "IST" "TID".
+    cStepsT. yield_tac "IST" "TID". yield_tac "IST" "TID".
     iApply wsim_mem_alloc; [try by simpl_map|ss|try lia|].
     replace (Z.to_nat (2 + sz)) with (2 + sz) by lia.
     iIntros (blk); rewrite replicate_add big_sepL_app; iIntros "[[sz [back _]] ar]". cStepsT.
-    sYieldIR "IST" "TID". sYieldIR "IST" "TID".
-    mStoreT "sz". sYieldIR "IST" "TID".
-    mStoreT "back". sYieldIR "IST" "TID".
+    yield_tac "IST" "TID". yield_tac "IST" "TID".
+    mStoreT "sz". yield_tac "IST" "TID".
+    mStoreT "back". yield_tac "IST" "TID".
     replace sz with ((sz - sz) + sz) at 1 by lia. rewrite replicate_add.
     replace (replicate (sz - sz) Vundef) with (replicate (sz - sz) (Vint 0))
       by rewrite Nat.sub_diag //=.
@@ -62,8 +49,8 @@ Section HWQPM.
     generalize sz at 1 4 5 10 as i; intros i Hle.
     iInduction i as [|i] forall (Hle st_src st_tgt).
     { rewrite Nat.sub_0_r /= app_nil_r.
-      unfoldIterT. cStepsT. sYieldIR "IST" "TID".
-      rewrite Nat2Z.id Nat.ltb_irrefl. cStepsT. sYieldIR "IST" "TID".
+      unfoldIterT. cStepsT. yield_tac "IST" "TID".
+      rewrite Nat2Z.id Nat.ltb_irrefl. cStepsT. yield_tac "IST" "TID".
       iDestruct "IST" as "[% [% [% [% [[-> ->] [[% IST] ->]]]]]]".
       iDestruct "IST" as "[IST [%X [free alloc]]]".
       destruct (decide (Vptr (blk, 0%Z) ∈ X)) as [HblkX|HblkX].
@@ -135,7 +122,7 @@ Section HWQPM.
       cStep. iFrame. auto.
     }
     (* inductive case *)
-    unfoldIterT. cStepsT. sYieldIR "IST" "TID".
+    unfoldIterT. cStepsT. yield_tac "IST" "TID".
     destruct Nat.ltb eqn : Hltb; first clear Hltb; last first.
     { apply Nat.ltb_ge in Hltb; lia. }
     iPoseProof (big_sepL_insert_acc _ _ (sz - (S i)) with "ar") as "[↦ ar]".
