single_coin/SingleCoinP.v
@@ -15,7 +15,7 @@ Module SingleCoinP. Section SingleCoinP.
     λ _,
       'cs : list (option bool) <- cgetU v_coins;;
       cput v_coins (cs ++ [None])%list;;;
-      ccallU (Y:=unit) (ProphecyName.new mn) (proph_coins (List.length cs));;;
+      ccallU (Y:=unit) (Prophecy.new mn) (proph_coins (List.length cs));;;
       Ret (List.length cs).
 
   Definition read : nat → itree crisE bool :=
@@ -26,7 +26,7 @@ Module SingleCoinP. Section SingleCoinP.
       | Some None =>
           b <- trigger (Choose bool);;
           cput v_coins ((firstn idx cs) ++ [Some b] ++ (skipn (S idx) cs))%list;;;
-          ccallU (Y:=unit) (ProphecyName.resolve mn) (proph_coins idx, b↑↑);;;
+          ccallU (Y:=unit) (Prophecy.resolve mn) (proph_coins idx, b↑↑);;;
           Ret b
       | None => triggerUB
       end.
